use nat addr in FSLayout

src/FSLayout.v
@@ -8,6 +8,8 @@ Require Import Arith.
 Require Import Hoare.
 Require Import SepAuto.
 Require Import Cache.
+Require Import AsyncDisk.
+Require Import Omega.
 
 Import ListNotations.
 Set Implicit Arguments.
@@ -40,6 +42,48 @@ Record fs_xparams := {
   FSXPRootInum : addr;
   FSXPMaxBlock : addr
 }.
+
+Definition log_xparams_ok xp :=
+  goodSize addrlen (DataStart xp) /\
+  goodSize addrlen (LogHeader xp) /\
+  goodSize addrlen ((LogDescriptor xp) + (LogDescLen xp)) /\
+  goodSize addrlen ((LogData xp) + (LogLen xp)).
+
+Definition balloc_xparams_ok xp :=
+  goodSize addrlen ((BmapStart xp) + (BmapNBlocks xp)).
+
+Definition inode_xparams_ok xp :=
+  goodSize addrlen ((IXStart xp) + (IXLen xp)).
+
+Definition fs_xparams_ok xp :=
+  log_xparams_ok (FSXPLog xp) /\
+  inode_xparams_ok (FSXPInode xp) /\
+  balloc_xparams_ok (FSXPBlockAlloc xp) /\
+  balloc_xparams_ok (FSXPInodeAlloc xp) /\
+  goodSize addrlen (FSXPRootInum xp) /\
+  goodSize addrlen (FSXPMaxBlock xp).
+
+Lemma goodSize_add_l : forall sz a b,
+  goodSize sz (a + b) -> goodSize sz a.
+Proof.
+  intros; eapply goodSize_trans with (n2 := a + b); auto; omega.
+Qed.
+
+Lemma goodSize_add_r : forall sz a b,
+  goodSize sz (a + b) -> goodSize sz b.
+Proof.
+  intros; eapply goodSize_trans with (n2 := a + b); auto; omega.
+Qed.
+
+Local Hint Resolve goodSize_add_l goodSize_add_r.
+
+Ltac xparams_ok := 
+  match goal with 
+  | [ H: fs_xparams_ok ?xp |- goodSize _ _ ] =>
+    unfold fs_xparams_ok, log_xparams_ok, balloc_xparams_ok, inode_xparams_ok in H;
+    intuition; eauto
+  end.
+
 
 Definition superblock_type : Rec.type := Rec.RecF ([
     ("data_start",  Rec.WordF addrlen);
@@ -76,41 +120,47 @@ Qed.
 Definition superblock0 := @Rec.of_word superblock_type (wzero _).
 Definition superblock_pad0 := @Rec.of_word superblock_padded (wzero _).
 
+Definition addr2w (a : addr) : waddr := natToWord addrlen a.
+
 Definition pickle_superblock (fsxp : fs_xparams) : word (Rec.len superblock_padded) :=
+  Eval compute_rec in
   let (lxp, ixp, ibxp, dbxp, rootinum, maxblock) := fsxp in
   let sb := superblock0
-    :=> "data_start"  := (DataStart lxp)
-    :=> "log_header"  := (LogHeader lxp)
-    :=> "log_descr"   := (LogDescriptor lxp)
-    :=> "log_data"    := (LogData lxp)
-    :=> "log_len"     := (LogLen lxp)
-    :=> "ixstart"     := (IXStart ixp)
-    :=> "ixlen"       := (IXLen ixp)
-    :=> "bastart"     := (BmapStart dbxp)
-    :=> "banblocks"   := (BmapNBlocks dbxp)
-    :=> "iastart"     := (BmapStart ibxp)
-    :=> "ianblocks"   := (BmapNBlocks ibxp)
-    :=> "root_inum"   := rootinum
-    :=> "maxblock"    := maxblock
+    :=> "data_start"  := addr2w (DataStart lxp)
+    :=> "log_header"  := addr2w (LogHeader lxp)
+    :=> "log_descr"   := addr2w (LogDescriptor lxp)
+    :=> "log_descrlen":= addr2w (LogDescLen lxp)
+    :=> "log_data"    := addr2w (LogData lxp)
+    :=> "log_len"     := addr2w (LogLen lxp)
+    :=> "ixstart"     := addr2w (IXStart ixp)
+    :=> "ixlen"       := addr2w (IXLen ixp)
+    :=> "bastart"     := addr2w (BmapStart dbxp)
+    :=> "banblocks"   := addr2w (BmapNBlocks dbxp)
+    :=> "iastart"     := addr2w (BmapStart ibxp)
+    :=> "ianblocks"   := addr2w (BmapNBlocks ibxp)
+    :=> "root_inum"   := addr2w rootinum
+    :=> "maxblock"    := addr2w maxblock
   in Rec.to_word (superblock_pad0 :=> "sb" := sb).
 
 Definition unpickle_superblock (sbp : word (Rec.len superblock_padded)) : fs_xparams :=
+  Eval compute_rec in
   let sb := ((Rec.of_word sbp) :-> "sb") in
   let lxp := Build_log_xparams
-    (sb :-> "data_start") (sb :-> "log_header")
-    (sb :-> "log_descr") (sb :-> "log_descrlen")
-    (sb :-> "log_data") (sb :-> "log_len") in
+    # (sb :-> "data_start") # (sb :-> "log_header")
+    # (sb :-> "log_descr") # (sb :-> "log_descrlen")
+    # (sb :-> "log_data") # (sb :-> "log_len") in
   let ixp := Build_inode_xparams
-    (sb :-> "ixstart") (sb :-> "ixlen") in
+    # (sb :-> "ixstart") # (sb :-> "ixlen") in
   let dbxp := Build_balloc_xparams
-    (sb :-> "bastart") (sb :-> "banblocks") in
+    # (sb :-> "bastart") # (sb :-> "banblocks") in
   let ibxp := Build_balloc_xparams
-    (sb :-> "iastart") (sb :-> "ianblocks") in
-  let rootinum := (sb :-> "root_inum") in
-  let maxblock := (sb :-> "maxblock") in
+    # (sb :-> "iastart") # (sb :-> "ianblocks") in
+  let rootinum := # (sb :-> "root_inum") in
+  let maxblock := # (sb :-> "maxblock") in
   Build_fs_xparams lxp ixp ibxp dbxp rootinum maxblock.
 
 Theorem pickle_unpickle_superblock : forall fsxp,
+  fs_xparams_ok fsxp ->
   unpickle_superblock (pickle_superblock fsxp) = fsxp.
 Proof.
   unfold pickle_superblock, unpickle_superblock.
@@ -121,9 +171,9 @@ Proof.
   destruct FSXPInodeAlloc0.
   destruct FSXPBlockAlloc0.
   unfold Rec.recget', Rec.recset'.
-  simpl.
-  reflexivity.
-
+  unfold addr2w; simpl; intros.
+  repeat rewrite wordToNat_natToWord_idempotent' by xparams_ok.
+  auto.
   unfold Rec.well_formed.
   simpl.
   intuition.
@@ -141,6 +191,7 @@ Definition v_unpickle_superblock (v : valu) : fs_xparams.
 Defined.
 
 Theorem v_pickle_unpickle_superblock : forall fsxp,
+  fs_xparams_ok fsxp ->
   v_unpickle_superblock (v_pickle_superblock fsxp) = fsxp.
 Proof.
   intros.
@@ -148,14 +199,14 @@ Proof.
   unfold eq_rec_r, eq_rec.
   rewrite eq_rect_nat_double.
   rewrite <- (eq_rect_eq_dec eq_nat_dec).
-  apply pickle_unpickle_superblock.
+  apply pickle_unpickle_superblock; auto.
 Qed.
 
-Definition sb_rep (fsxp : fs_xparams) : @pred _ (@weq addrlen) _ :=
-  ($0 |=> v_pickle_superblock fsxp)%pred.
+Definition sb_rep (fsxp : fs_xparams) : rawpred :=
+  ([[ fs_xparams_ok fsxp ]] * 0 |=> v_pickle_superblock fsxp)%pred.
 
 Definition sb_load T cs rx : prog T :=
-  let^ (cs, v) <- BUFCACHE.read $0 cs;
+  let^ (cs, v) <- BUFCACHE.read 0 cs;
   rx ^(cs, v_unpickle_superblock v).
 
 Theorem sb_load_ok : forall cs,
@@ -170,23 +221,23 @@ Theorem sb_load_ok : forall cs,
 Proof.
   unfold sb_load, sb_rep.
   hoare.
-  subst; apply v_pickle_unpickle_superblock.
+  subst; apply v_pickle_unpickle_superblock; auto.
 Qed.
 
 Definition sb_init T fsxp cs rx : prog T :=
-  cs <- BUFCACHE.write $0 (v_pickle_superblock fsxp) cs;
-  cs <- BUFCACHE.sync $0 cs;
+  cs <- BUFCACHE.write 0 (v_pickle_superblock fsxp) cs;
+  cs <- BUFCACHE.sync 0 cs;
   rx cs.
 
 Theorem sb_init_ok : forall fsxp cs,
   {< m F,
   PRE
-    BUFCACHE.rep cs m * [[ (F * $0 |->?)%pred m ]]
+    BUFCACHE.rep cs m * [[ fs_xparams_ok fsxp /\ (F * 0 |->?)%pred m ]]
   POST RET:cs
     exists m',
     BUFCACHE.rep cs m' * [[ (F * sb_rep fsxp)%pred m' ]]
   CRASH
-    exists cs' m', BUFCACHE.rep cs' m' * [[ (F * $0 |->?)%pred m' ]]
+    exists cs' m', BUFCACHE.rep cs' m' * [[ (F * 0 |->?)%pred m' ]]
   >} sb_init fsxp cs.
 Proof.
   unfold sb_rep, sb_init.
